src/go_lang/lib/lock.v
@@ -1,0 +1,38 @@
+From iris.base_logic.lib Require Export invariants.
+From Perennial.go_lang Require Export lifting notation.
+Set Default Proof Using "Type".
+
+Structure lock `{ffi_sem: ext_semantics} Σ `{!heapG Σ} := Lock {
+  (* -- operations -- *)
+  newlock : val;
+  acquire : val;
+  release : val;
+  (* -- predicates -- *)
+  (* name is used to associate locked with is_lock *)
+  name : Type;
+  is_lock (N: namespace) (γ: name) (lock: val) (R: iProp Σ) : iProp Σ;
+  locked (γ: name) : iProp Σ;
+  (* -- general properties -- *)
+  is_lock_ne N γ lk : NonExpansive (is_lock N γ lk);
+  is_lock_persistent N γ lk R : Persistent (is_lock N γ lk R);
+  locked_timeless γ : Timeless (locked γ);
+  locked_exclusive γ : locked γ -∗ locked γ -∗ False;
+  (* -- operation specs -- *)
+  newlock_spec N (R : iProp Σ) :
+    {{{ R }}} newlock #() {{{ lk γ, RET lk; is_lock N γ lk R }}};
+  acquire_spec N γ lk R :
+    {{{ is_lock N γ lk R }}} acquire lk {{{ RET #(); locked γ ∗ R }}};
+  release_spec N γ lk R :
+    {{{ is_lock N γ lk R ∗ locked γ ∗ R }}} release lk {{{ RET #(); True }}}
+}.
+
+Arguments newlock {_ _ _ _ _} l.
+Arguments acquire {_ _ _ _ _} l.
+Arguments release {_ _ _ _ _} l.
+Arguments is_lock {_ _ _ _ _} l _ _ _ _.
+Arguments locked {_ _ _ _ _} l _.
+
+Existing Instances is_lock_ne is_lock_persistent locked_timeless.
+
+Instance is_lock_proper `{ffi_sem: ext_semantics} Σ `{!heapG Σ} (L: lock Σ) N γ lk:
+  Proper ((≡) ==> (≡)) (is_lock L N γ lk) := ne_proper _.
