src/go_lang/lib/spin_lock.v
@@ -1,0 +1,105 @@
+From iris.proofmode Require Import tactics.
+From iris.algebra Require Import excl.
+From iris.program_logic Require Export weakestpre.
+From Perennial.go_lang Require Export lang.
+From Perennial.go_lang Require Import proofmode notation.
+From Perennial.go_lang.lib Require Import lock.
+Set Default Proof Using "Type".
+
+Section go_lang.
+  Context `{ffi_sem: ext_semantics}.
+
+  (* Coercion Var : string >-> expr. *)
+  Definition Var' s : @expr ext := Var s.
+  Coercion Var' : string >-> expr.
+
+Definition newlock : val := λ: <>, ref #false.
+Definition try_acquire : val := λ: "l", CAS "l" #false #true.
+Definition acquire : val :=
+  rec: "acquire" "l" := if: try_acquire "l" then #() else "acquire" "l".
+Definition release : val := λ: "l", "l" <- #false.
+
+(** The CMRA we need. *)
+(* Not bundling heapG, as it may be shared with other users. *)
+Class lockG Σ := LockG { lock_tokG :> inG Σ (exclR unitO) }.
+Definition lockΣ : gFunctors := #[GFunctor (exclR unitO)].
+
+Instance subG_lockΣ {Σ} : subG lockΣ Σ → lockG Σ.
+Proof. solve_inG. Qed.
+
+Section proof.
+  Context `{!heapG Σ, !lockG Σ} (N : namespace).
+
+  Definition lock_inv (γ : gname) (l : loc) (R : iProp Σ) : iProp Σ :=
+    (∃ b : bool, l ↦ #b ∗ if b then True else own γ (Excl ()) ∗ R)%I.
+
+  Definition is_lock (γ : gname) (lk : val) (R : iProp Σ) : iProp Σ :=
+    (∃ l: loc, ⌜lk = #l⌝ ∧ inv N (lock_inv γ l R))%I.
+
+  Definition locked (γ : gname) : iProp Σ := own γ (Excl ()).
+
+  Lemma locked_exclusive (γ : gname) : locked γ -∗ locked γ -∗ False.
+  Proof. iIntros "H1 H2". by iDestruct (own_valid_2 with "H1 H2") as %?. Qed.
+
+  Global Instance lock_inv_ne γ l : NonExpansive (lock_inv γ l).
+  Proof. solve_proper. Qed.
+  Global Instance is_lock_ne γ l : NonExpansive (is_lock γ l).
+  Proof. solve_proper. Qed.
+
+  (** The main proofs. *)
+  Global Instance is_lock_persistent γ l R : Persistent (is_lock γ l R).
+  Proof. apply _. Qed.
+  Global Instance locked_timeless γ : Timeless (locked γ).
+  Proof. apply _. Qed.
+
+  Lemma newlock_spec (R : iProp Σ):
+    {{{ R }}} newlock #() {{{ lk γ, RET lk; is_lock γ lk R }}}.
+  Proof.
+    iIntros (Φ) "HR HΦ". rewrite -wp_fupd /newlock /=.
+    wp_lam. wp_alloc l as "Hl".
+    iMod (own_alloc (Excl ())) as (γ) "Hγ"; first done.
+    iMod (inv_alloc N _ (lock_inv γ l R) with "[-HΦ]") as "#?".
+    { iIntros "!>". iExists false. by iFrame. }
+    iModIntro. iApply "HΦ". iExists l. eauto.
+  Qed.
+
+  Lemma try_acquire_spec γ lk R :
+    {{{ is_lock γ lk R }}} try_acquire lk
+    {{{ b, RET #b; if b is true then locked γ ∗ R else True }}}.
+  Proof.
+    iIntros (Φ) "#Hl HΦ". iDestruct "Hl" as (l ->) "#Hinv".
+    wp_rec.
+    wp_bind (CmpXchg _ _ _). iInv N as ([]) "[Hl HR]".
+    - wp_cmpxchg_fail. iModIntro. iSplitL "Hl"; first (iNext; iExists true; eauto).
+      wp_pures. iApply ("HΦ" $! false). done.
+    - wp_cmpxchg_suc. iDestruct "HR" as "[Hγ HR]".
+      iModIntro. iSplitL "Hl"; first (iNext; iExists true; eauto).
+      rewrite /locked. wp_pures. by iApply ("HΦ" $! true with "[$Hγ $HR]").
+  Qed.
+
+  Lemma acquire_spec γ lk R :
+    {{{ is_lock γ lk R }}} acquire lk {{{ RET #(); locked γ ∗ R }}}.
+  Proof.
+    iIntros (Φ) "#Hl HΦ". iLöb as "IH". wp_rec.
+    wp_apply (try_acquire_spec with "Hl"). iIntros ([]).
+    - iIntros "[Hlked HR]". wp_if. iApply "HΦ"; iFrame.
+    - iIntros "_". wp_if. iApply ("IH" with "[HΦ]"). auto.
+  Qed.
+
+  Lemma release_spec γ lk R :
+    {{{ is_lock γ lk R ∗ locked γ ∗ R }}} release lk {{{ RET #(); True }}}.
+  Proof.
+    iIntros (Φ) "(Hlock & Hlocked & HR) HΦ".
+    iDestruct "Hlock" as (l ->) "#Hinv".
+    rewrite /release /=. wp_lam. iInv N as (b) "[Hl _]".
+    wp_store. iSplitR "HΦ"; last by iApply "HΦ".
+    iModIntro. iNext. iExists false. by iFrame.
+  Qed.
+End proof.
+End go_lang.
+
+Typeclasses Opaque is_lock locked.
+
+Canonical Structure spin_lock `{ffi_sem: ext_semantics} `{!heapG Σ, !lockG Σ} : lock Σ :=
+  {| lock.locked_exclusive := locked_exclusive; lock.newlock_spec := newlock_spec;
+     lock.acquire_spec := acquire_spec; lock.release_spec := release_spec |}.
