src/go_lang/notation.v
@@ -18,7 +18,7 @@ Coercion LitProphecy : proph_id >-> base_lit.
 Coercion App : expr >-> Funclass.
 
 Coercion Val : val >-> expr.
-Coercion Var : string >-> expr.
+(* Coercion Var : string >-> expr. *)
 
 (** Define some derived forms. *)
 Notation Lam x e := (Rec BAnon x e) (only parsing).
